invariants

dp/6_4.dfy
@@ -15,9 +15,39 @@ module SixFour {
         || a == "the"
     }
 
+    predicate method methDict(a: string)
+    {
+        a == "a" 
+        || a == "as"
+        || a == "the"
+    }
+
     // Needs to be <= O(n^2).
     method greedySixFour(a: string) returns (words: bool)
+    requires |a|>0
     {
+        if |a|==1 { return methDict(a); }
+        var p := "\0" + a;
+
+        var ar := new bool[|p|];
+        ar[0] := true;
+        var i := 1;
+
+        while i < ar.Length 
+        invariant 0<i<=|p|
+        invariant 0<i<=ar.Length
+        invariant |p|>2
+        invariant ar.Length>2
+        decreases ar.Length - i
+        {
+            if methDict([p[i]]) {
+                ar[i] := true;
+            } else {
+
+            }
+            i := i+1;
+        }
+
         return false;
     }
 
